include/pulse/Pulse.Lib.C.Casts.fst
@@ -1,10 +1,25 @@
 module Pulse.Lib.C.Casts
 #lang-pulse
 open Pulse
-include FStar.SizeT
-include FStar.Int.Cast
 
-let int32_to_sizet (x: FStar.Int32.t {FStar.Int32.gte x 0l}) =
-  let u = int32_to_uint32 x in
-  assume (SizeT.fits_u32);
-  uint32_to_sizet u
+open Pulse.Lib.C.Assumptions
+
+module C = FStar.Int.Cast
+
+let int32_to_sizet (x: Int32.t) =
+  let u = C.int32_to_uint32 x in
+  SizeT.uint32_to_sizet u
+
+let int64_to_sizet (x: Int64.t) =
+  let u = C.int64_to_uint64 x in
+  SizeT.uint64_to_sizet u
+
+// NB: The deprecation warning below is spurious, we will
+// not overflow the signed int due to our precondition.
+let sizet_to_int32 (x: SizeT.t) =
+  let u = SizeT.sizet_to_uint32 x in
+  C.uint32_to_int32 u
+
+let sizet_to_int64 (x: SizeT.t) =
+  let u = SizeT.sizet_to_uint64 x in
+  C.uint64_to_int64 u
